Veir/Data/LLVM/Byte/Lemmas.lean
@@ -7,14 +7,13 @@ namespace Veir.Data.LLVM.Byte
 open Veir.Data.LLVM.Int
 
 theorem toInt_fromInt {w : Nat} (x : Int w) (h : 0 < w) : (Byte.fromInt x).toInt = x := by
-  simp only [Byte.toInt, fromInt]
+  simp only [Byte.toInt]
   cases x
-  · simp
-  · have := Nat.two_pow_pred_lt_two_pow h
-    have := Nat.two_pow_pos (w-1)
-    rw [ite_eq_right_iff, BitVec.toNat_eq]
-    simp
+  case poison =>
+    simp [fromInt, ← BitVec.neg_one_eq_allOnes]
     omega
+  case value v =>
+    simp [fromInt]
 
 @[bv_normalize]
 theorem ext_iff {w : Nat} (x y : Byte w) :
